mppa_k1c/abstractbb/SeqSimuTheory.v
@@ -3,103 +3,89 @@
 *)
 
 
+Require Coq.Logic.FunctionalExtensionality. (* not really necessary -- see lemma at the end *)
 Require Setoid. (* in order to rewrite <-> *)
 Require Export AbstractBasicBlocksDef.
 Require Import List.
 Require Import ImpPrelude.
 Import HConsingDefs.
 
-Module Type PseudoRegDictionary.
 
-Declare Module R: PseudoRegisters.
-
-Parameter t: Type -> Type.
-
-Parameter get: forall {A}, t A -> R.t -> option A.
-
-Parameter set: forall {A}, t A -> R.t -> A -> t A.
-
-Parameter set_spec_eq: forall A d x (v: A),
-  get (set d x v) x = Some v.
-
-Parameter set_spec_diff: forall A d x y (v: A),
-  x <> y -> get (set d x v) y = get d y.
-
-Parameter empty: forall {A}, t A.
-
-Parameter empty_spec: forall A x,
-  get (empty (A:=A)) x = None.
-
-End PseudoRegDictionary.
-
-
-Module SimuTheory (L: SeqLanguage) (Dict: PseudoRegDictionary with Module R:=L.LP.R).
+Module SimuTheory (L: SeqLanguage).
 
 Export L.
 Export LP.
-Export Terms.
+
+Inductive term :=
+  | Input (x:R.t)
+  | App (o: op) (l: list_term)
+with list_term :=
+  | LTnil
+  | LTcons (t:term) (l:list_term)
+  .
+
+Fixpoint term_eval (ge: genv) (t: term) (m: mem): option value :=
+  match t with
+  | Input x => Some (m x)
+  | App o l =>
+     match list_term_eval ge l m with
+     | Some v => op_eval ge o v
+     | _ => None
+     end
+  end
+with list_term_eval ge (l: list_term) (m: mem) {struct l}: option (list value) :=
+  match l with
+  | LTnil => Some nil
+  | LTcons t l' => 
+    match term_eval ge t m, list_term_eval ge l' m with
+    | Some v, Some lv => Some (v::lv)
+    | _, _ => None
+    end
+  end.
 
 (* the symbolic memory:
   - pre: pre-condition expressing that the computation has not yet abort on a None.
   - post: the post-condition for each pseudo-register 
 *)
-Record smem:= {pre: genv -> mem -> Prop; post: Dict.t term}.
-
-Coercion post: smem >-> Dict.t.
+Record smem:= {pre: genv -> mem -> Prop; post:> R.t -> term}.
 
 (** initial symbolic memory *)
-Definition smem_empty := {| pre:=fun _ _ => True; post:=Dict.empty |}.
+Definition smem_empty := {| pre:=fun _ _ => True; post:=(fun x => Input x) |}.
 
-Definition smem_get (d:Dict.t term) x := 
-   match Dict.get d x with 
-   | None => Input x unknown_hid
-   | Some t => t
-   end.
-
-Fixpoint exp_term (e: exp) (d old: Dict.t term): term :=
+Fixpoint exp_term (e: exp) (d old: smem) : term :=
   match e with
-  | PReg x => smem_get d x
-  | Op o le => App o (list_exp_term le d old) unknown_hid
+  | PReg x => d x
+  | Op o le => App o (list_exp_term le d old)
   | Old e => exp_term e old old
   end
-with list_exp_term (le: list_exp) (d old: Dict.t term) : list_term :=
+with list_exp_term (le: list_exp) (d old: smem) : list_term :=
   match le with
-  | Enil => LTnil unknown_hid
-  | Econs e le' => LTcons (exp_term e d old) (list_exp_term le' d old) unknown_hid
+  | Enil => LTnil
+  | Econs e le' => LTcons (exp_term e d old) (list_exp_term le' d old)
   | LOld le => list_exp_term le old old
   end.
 
-(** evaluation of the post-condition *)
-Definition smem_eval ge (d: Dict.t term) x (m:mem) :=
-  term_eval ge (smem_get d x) m.
 
 (** assignment of the symbolic memory *)
 Definition smem_set (d:smem) x (t:term) := 
-  {| pre:=(fun ge m => (smem_eval ge d x m) <> None /\ (d.(pre) ge m));
-     post:=Dict.set d x t |}.
+  {| pre:=(fun ge m => (term_eval ge (d x) m) <> None /\ (d.(pre) ge m));
+     post:=fun y => if R.eq_dec x y then t else d y |}.
 
 Section SIMU_THEORY.
 
 Variable ge: genv.
 
 Lemma set_spec_eq d x t m:
- smem_eval ge (smem_set d x t) x m = term_eval ge t m.
+ term_eval ge (smem_set d x t x) m = term_eval ge t m.
 Proof.
-  unfold smem_eval, smem_set, smem_get; simpl; rewrite Dict.set_spec_eq; simpl; auto. 
+  unfold smem_set; simpl; case (R.eq_dec x x); try congruence.
 Qed.
 
 Lemma set_spec_diff d x y t m:
-  x <> y -> smem_eval ge (smem_set d x t) y m = smem_eval ge d y m.
+  x <> y -> term_eval ge (smem_set d x t y) m = term_eval ge (d y) m.
 Proof.
-  intros; unfold smem_eval, smem_set, smem_get; simpl; rewrite Dict.set_spec_diff; simpl; auto. 
+  unfold smem_set; simpl; case (R.eq_dec x y); try congruence.
 Qed.
-
-Lemma smem_eval_empty x m: smem_eval ge smem_empty x m = Some (m x).
-Proof.
-  unfold smem_eval, smem_get; rewrite Dict.empty_spec; simpl; auto.
-Qed.
-
-Hint Rewrite set_spec_eq smem_eval_empty: dict_rw. 
 
 Fixpoint inst_smem (i: inst) (d old: smem): smem :=
   match i with
@@ -116,8 +102,9 @@ Fixpoint bblock_smem_rec (p: bblock) (d: smem): smem :=
      let d':=inst_smem i d d in
      bblock_smem_rec p' d'
   end.
-
+(*
 Local Hint Resolve smem_eval_empty.
+*)
 
 Definition bblock_smem: bblock -> smem
  := fun p => bblock_smem_rec p smem_empty.
@@ -140,37 +127,36 @@ Qed.
 Local Hint Resolve inst_smem_pre_monotonic bblock_smem_pre_monotonic.
 
 Lemma term_eval_exp e (od:smem) m0 old:
-  (forall x, smem_eval ge od x m0 = Some (old x)) ->
-  forall d m1,
-   (forall x, smem_eval ge (d:smem) x m0 = Some (m1 x)) ->
+  (forall x, term_eval ge (od x) m0 = Some (old x)) ->
+  forall (d:smem) m1,
+   (forall x, term_eval ge (d x) m0 = Some (m1 x)) ->
     term_eval ge (exp_term e d od) m0 = exp_eval ge e m1 old.
 Proof.
-  unfold smem_eval in * |- *; intro H.
+  intro H.
   induction e using exp_mut with
-    (P0:=fun l => forall (d:smem) m1, (forall x, term_eval ge (smem_get d x) m0 = Some (m1 x)) -> list_term_eval ge (list_exp_term l d od) m0 = list_exp_eval ge l m1 old);
+    (P0:=fun l => forall (d:smem) m1, (forall x, term_eval ge (d x) m0 = Some (m1 x)) -> list_term_eval ge (list_exp_term l d od) m0 = list_exp_eval ge l m1 old);
   simpl; auto.
   - intros; erewrite IHe; eauto.
   - intros. erewrite IHe, IHe0; eauto. 
 Qed.
 
-Lemma inst_smem_abort i m0 x old: forall d,
+Lemma inst_smem_abort i m0 x old: forall (d:smem),
     pre (inst_smem i d old) ge m0 ->
-    smem_eval ge d x m0 = None ->
-    smem_eval ge (inst_smem i d old) x m0 = None.
+    term_eval ge (d x) m0 = None ->
+    term_eval ge (inst_smem i d old x) m0 = None.
 Proof.
   induction i as [|[y e] i IHi]; simpl; auto.
   intros d VALID H; erewrite IHi; eauto. clear IHi.
-  destruct (R.eq_dec x y).
-  * subst; autorewrite with dict_rw.
-    generalize (inst_smem_pre_monotonic _ _ _ _ VALID); clear VALID.
-    unfold smem_set; simpl; intuition congruence.
-  * rewrite set_spec_diff; auto.
+  unfold smem_set; simpl; destruct (R.eq_dec y x); auto.
+  subst;
+  generalize (inst_smem_pre_monotonic _ _ _ _ VALID); clear VALID.
+  unfold smem_set; simpl. intuition congruence.
 Qed.
 
 Lemma block_smem_rec_abort p m0 x: forall d,
     pre (bblock_smem_rec p d) ge m0 ->
-    smem_eval ge d x m0 = None ->
-    smem_eval ge (bblock_smem_rec p d) x m0 = None.
+    term_eval ge (d x) m0 = None ->
+    term_eval ge (bblock_smem_rec p d x) m0 = None.
 Proof.
   induction p; simpl; auto.
   intros d VALID H; erewrite IHp; eauto. clear IHp.
@@ -178,11 +164,11 @@ Proof.
 Qed.
 
 Lemma inst_smem_Some_correct1 i m0 old (od:smem): 
-  (forall x, smem_eval ge od x m0 = Some (old x)) ->
+  (forall x, term_eval ge (od x) m0 = Some (old x)) ->
   forall (m1 m2: mem) (d: smem), 
   inst_run ge i m1 old = Some m2 -> 
-  (forall x, smem_eval ge d x m0 = Some (m1 x)) ->
-   forall x, smem_eval ge (inst_smem i d od) x m0 = Some (m2 x).
+  (forall x, term_eval ge (d x) m0 = Some (m1 x)) ->
+   forall x, term_eval ge (inst_smem i d od x) m0 = Some (m2 x).
 Proof.
   intro X; induction i as [|[x e] i IHi]; simpl; intros m1 m2 d H.
   - inversion_clear H; eauto.
@@ -190,16 +176,14 @@ Proof.
     destruct (exp_eval ge e m1 old) eqn:Heqov; try congruence.
     refine (IHi _ _ _ _ _ _); eauto.
     clear x0; intros x0.
-    unfold assign; destruct (R.eq_dec x x0).
-    * subst; autorewrite with dict_rw.
-      erewrite term_eval_exp; eauto.
-    * rewrite set_spec_diff; auto.
+    unfold assign, smem_set; simpl. destruct (R.eq_dec x x0); auto.
+    subst; erewrite term_eval_exp; eauto.
 Qed.
 
 Lemma bblocks_smem_rec_Some_correct1 p m0: forall (m1 m2: mem) (d: smem), 
  run ge p m1 = Some m2 -> 
-  (forall x, smem_eval ge d x m0 = Some (m1 x)) ->
-  forall x, smem_eval ge (bblock_smem_rec p d) x m0 = Some (m2 x).
+  (forall x, term_eval ge (d x) m0 = Some (m1 x)) ->
+  forall x, term_eval ge (bblock_smem_rec p d x) m0 = Some (m2 x).
 Proof.
   Local Hint Resolve inst_smem_Some_correct1.
   induction p as [ | i p]; simpl; intros m1 m2 d H.
@@ -212,39 +196,37 @@ Qed.
 
 Lemma bblock_smem_Some_correct1 p m0 m1:
    run ge p m0 = Some m1
-   -> forall x, smem_eval ge (bblock_smem p) x m0 = Some (m1 x).
+   -> forall x, term_eval ge (bblock_smem p x) m0 = Some (m1 x).
 Proof.
   intros; eapply bblocks_smem_rec_Some_correct1; eauto.
 Qed.
 
 Lemma inst_smem_None_correct i m0 old (od: smem):
-   (forall x, smem_eval ge od x m0 = Some (old x)) ->
+   (forall x, term_eval ge (od x) m0 = Some (old x)) ->
   forall m1 d, pre (inst_smem i d od) ge m0 ->
-   (forall x, smem_eval ge d x m0 = Some (m1 x)) ->
-  inst_run ge i m1 old = None -> exists x, smem_eval ge (inst_smem i d od) x m0 = None.
+   (forall x, term_eval ge (d x) m0 = Some (m1 x)) ->
+  inst_run ge i m1 old = None -> exists x, term_eval ge (inst_smem i d od x) m0 = None.
 Proof.
   intro X; induction i as [|[x e] i IHi]; simpl; intros m1 d.
   - discriminate.
   - intros VALID H0.
     destruct (exp_eval ge e m1 old) eqn: Heqov.
     + refine (IHi _ _ _ _); eauto.
-      intros x0; unfold assign; destruct (R.eq_dec x x0).
-      * subst; autorewrite with dict_rw. 
-        erewrite term_eval_exp; eauto.
-      * rewrite set_spec_diff; auto.
+      intros x0; unfold assign, smem_set; simpl. destruct (R.eq_dec x x0); auto.
+      subst; erewrite term_eval_exp; eauto.
     + intuition.
       constructor 1 with (x:=x); simpl.
       apply inst_smem_abort; auto.
-      autorewrite with dict_rw.
+      rewrite set_spec_eq. 
       erewrite term_eval_exp; eauto.
 Qed.
 
 Lemma inst_smem_Some_correct2 i m0 old (od: smem):
-  (forall x, smem_eval ge od x m0 = Some (old x)) ->
+  (forall x, term_eval ge (od x) m0 = Some (old x)) ->
   forall (m1 m2: mem) d, 
   pre (inst_smem i d od) ge m0 ->
-  (forall x, smem_eval ge d x m0 = Some (m1 x)) ->
-  (forall x, smem_eval ge (inst_smem i d od) x m0 = Some (m2 x)) ->
+  (forall x, term_eval ge (d x) m0 = Some (m1 x)) ->
+  (forall x, term_eval ge (inst_smem i d od x) m0 = Some (m2 x)) ->
   res_eq (Some m2) (inst_run ge i m1 old).
 Proof.
   intro X.
@@ -255,20 +237,18 @@ Proof.
   - intros H.
     destruct (exp_eval ge e m1 old) eqn: Heqov.
     + refine (IHi _ _ _ _ _ _); eauto.
-      intros x0; unfold assign; destruct (R.eq_dec x x0).
-      * subst. autorewrite with dict_rw.
-        erewrite term_eval_exp; eauto.
-      * rewrite set_spec_diff; auto.
+      intros x0; unfold assign, smem_set; simpl; destruct (R.eq_dec x x0); auto.
+      subst; erewrite term_eval_exp; eauto.
     + generalize (H x).
       rewrite inst_smem_abort; discriminate || auto.
-      autorewrite with dict_rw. 
+      rewrite set_spec_eq. 
       erewrite term_eval_exp; eauto.
 Qed.
 
 Lemma bblocks_smem_rec_Some_correct2 p m0: forall (m1 m2: mem) d, 
   pre (bblock_smem_rec p d) ge m0 ->
-  (forall x, smem_eval ge d x m0 = Some (m1 x)) ->
-  (forall x, smem_eval ge (bblock_smem_rec p d) x m0 = Some (m2 x)) ->
+  (forall x, term_eval ge (d x) m0 = Some (m1 x)) ->
+  (forall x, term_eval ge (bblock_smem_rec p d x) m0 = Some (m2 x)) ->
     res_eq (Some m2) (run ge p m1).
 Proof.
   induction p as [|i p]; simpl; intros m1 m2 d VALID H0.
@@ -278,7 +258,7 @@ Proof.
   - intros H.
      destruct (inst_run ge i m1 m1) eqn: Heqom.
     + refine (IHp _ _ _ _ _ _); eauto.
-    + assert (X: exists x, term_eval ge (smem_get (inst_smem i d d) x) m0 = None).
+    + assert (X: exists x, term_eval ge (inst_smem i d d x) m0 = None).
       { eapply inst_smem_None_correct; eauto. }
       destruct X as [x H1].
       generalize (H x).
@@ -286,21 +266,20 @@ Proof.
       congruence.
 Qed.
 
-
 Lemma bblock_smem_Some_correct2 p m0 m1:
   pre (bblock_smem p) ge m0 ->
-  (forall x, smem_eval ge (bblock_smem p) x m0 = Some (m1 x))
+  (forall x, term_eval ge (bblock_smem p x) m0 = Some (m1 x))
   -> res_eq (Some m1) (run ge p m0).
 Proof.
   intros; eapply bblocks_smem_rec_Some_correct2; eauto.
 Qed.
 
 Lemma inst_valid i m0 old (od:smem):
-  (forall x, smem_eval ge od x m0 = Some (old x)) ->
+  (forall x, term_eval ge (od x) m0 = Some (old x)) ->
   forall (m1 m2: mem) (d: smem), 
   pre d ge m0 ->
   inst_run ge i m1 old = Some m2 ->
-  (forall x, smem_eval ge d x m0 = Some (m1 x)) ->
+  (forall x, term_eval ge (d x) m0 = Some (m1 x)) ->
    pre (inst_smem i d od) ge m0.
 Proof.
   induction i as [|[x e] i IHi]; simpl; auto.
@@ -309,17 +288,15 @@ Proof.
   eapply IHi; eauto.
   + unfold smem_set in * |- *; simpl. 
     rewrite Hm1; intuition congruence.
-  + intros x0. unfold assign; destruct (R.eq_dec x x0).
-    * subst; autorewrite with dict_rw.
-      erewrite term_eval_exp; eauto.
-    * rewrite set_spec_diff; auto.
+  + intros x0. unfold assign, smem_set; simpl; destruct (R.eq_dec x x0); auto.
+    subst; erewrite term_eval_exp; eauto.
 Qed.
 
 
 Lemma block_smem_rec_valid p m0: forall (m1 m2: mem) (d:smem), 
   pre d ge m0 ->
   run ge p m1 = Some m2 -> 
-  (forall x, smem_eval ge d x m0 = Some (m1 x)) ->
+  (forall x, term_eval ge (d x) m0 = Some (m1 x)) ->
   pre (bblock_smem_rec p d) ge m0.
 Proof.
   Local Hint Resolve inst_valid.
@@ -337,22 +314,26 @@ Proof.
   unfold smem_empty; simpl. auto.
 Qed.
 
-Definition smem_valid ge d m := pre d ge m /\ forall x, smem_eval ge d x m <> None.
+Definition smem_valid ge d m := pre d ge m /\ forall x, term_eval ge (d x) m <> None.
+
+Definition smem_simu (d1 d2: smem): Prop :=
+     (forall m, smem_valid ge d1 m -> smem_valid ge d2 m)
+  /\ (forall m0 x, smem_valid ge d1 m0 -> 
+                   term_eval ge (d1 x) m0 = term_eval ge (d2 x) m0).
+
 
 Theorem bblock_smem_simu p1 p2:
-  (forall m, smem_valid ge (bblock_smem p1) m -> smem_valid ge (bblock_smem p2) m) ->
-  (forall m0 x m1, smem_valid ge (bblock_smem p1) m0 -> smem_eval ge (bblock_smem p1) x m0 = Some m1 ->
-                   smem_eval ge (bblock_smem p2) x m0 = Some m1) ->
+   smem_simu (bblock_smem p1) (bblock_smem p2) ->
    bblock_simu ge p1 p2.
 Proof.
   Local Hint Resolve bblock_smem_valid bblock_smem_Some_correct1.
-  unfold smem_valid; intros INCL EQUIV m DONTFAIL.
+  intros (INCL & EQUIV) m DONTFAIL; unfold smem_valid in * |-.
   destruct (run ge p1 m) as [m1|] eqn: RUN1; simpl; try congruence.
-  assert (X: forall x, smem_eval ge (bblock_smem p1) x m = Some (m1 x)); eauto.
+  assert (X: forall x, term_eval ge (bblock_smem p1 x) m = Some (m1 x)); eauto.
   eapply bblock_smem_Some_correct2; eauto.
   + destruct (INCL m); intuition eauto.
     congruence.
-  + intro x; apply EQUIV; intuition eauto.
+  + intro x; erewrite <- EQUIV; intuition eauto.
     congruence.
 Qed.
 
@@ -370,7 +351,7 @@ Lemma smem_valid_set_decompose_2 d t x m:
   smem_valid ge (smem_set d x t) m -> term_eval ge t m <> None.
 Proof.
   unfold smem_valid; intros ((PRE1 & PRE2) & VALID) H.
-  generalize (VALID x); autorewrite with dict_rw.
+  generalize (VALID x); rewrite set_spec_eq.
   tauto.
 Qed.
 
@@ -379,50 +360,28 @@ Lemma smem_valid_set_proof d x t m:
 Proof.
   unfold smem_valid; intros (PRE & VALID) PREt. split.
   + split; auto.
-  + intros x0; case (R.eq_dec x x0).
-    - intros; subst; autorewrite with dict_rw. auto.
-    - intros. rewrite set_spec_diff; auto. 
+  + intros x0; unfold smem_set; simpl; case (R.eq_dec x x0); intros; subst; auto.
 Qed.
+
 
 End SIMU_THEORY.
 
+(** REMARKS: more abstract formulation of the proof... 
+    but relying on functional_extensionality.
+*)
+Definition smem_correct ge (d: smem) (m: mem) (om: option mem): Prop:=
+   forall m', om=Some m' <-> (d.(pre) ge m /\ forall x, term_eval ge (d x) m = Some (m' x)).
+
+Lemma bblock_smem_correct ge p m: smem_correct ge (bblock_smem p) m (run ge p m).
+Proof.
+  unfold smem_correct; simpl; intros m'; split.
+  + intros; split.
+    * eapply bblock_smem_valid; eauto.
+    * eapply bblock_smem_Some_correct1; eauto.
+  + intros (H1 & H2).
+    destruct (bblock_smem_Some_correct2 ge p m m') as (m2 & X & Y); eauto.
+    rewrite X. f_equal.
+    apply FunctionalExtensionality.functional_extensionality; auto.
+Qed.
+
 End SimuTheory.
-
-Require Import PArith.
-Require Import FMapPositive.
-
-Module PosDict <: PseudoRegDictionary with Module R:=Pos.
-
-Module R:=Pos.
-
-Definition t:=PositiveMap.t.
-
-Definition get {A} (d:t A) (x:R.t): option A 
- := PositiveMap.find x d.
-
-Definition set {A} (d:t A) (x:R.t) (v:A): t A
- := PositiveMap.add x v d.
-
-Local Hint Unfold PositiveMap.E.eq.
-
-Lemma set_spec_eq A d x (v: A):
-  get (set d x v) x = Some v.
-Proof.
-  unfold get, set; apply PositiveMap.add_1; auto.
-Qed.
-
-Lemma set_spec_diff A d x y (v: A):
-  x <> y -> get (set d x v) y = get d y.
-Proof.
-  unfold get, set; intros; apply PositiveMap.gso; auto.
-Qed.
-
-Definition empty {A}: t A := PositiveMap.empty A.
-
-Lemma empty_spec A x:
-  get (empty (A:=A)) x = None.
-Proof.
-  unfold get, empty; apply PositiveMap.gempty; auto.
-Qed.
-
-End PosDict.
